BB52Statement.v
@@ -1,0 +1,74 @@
+Require Import ZArith.
+
+Inductive St:Set :=
+| St0
+| St1
+| St2
+| St3
+| St4.
+
+Inductive Σ:Set :=
+| Σ0
+| Σ1.
+
+Inductive Dir:Set :=
+| Dneg
+| Dpos.
+
+Definition Dir_to_Z(x:Dir) :=
+match x with
+| Dneg => Zneg 1
+| Dpos => Zpos 1
+end.
+
+Section TM.
+
+Hypothesis Σ:Set.
+Hypothesis Σ0:Σ.
+
+Record Trans:Set := {
+  nxt: St;
+  dir: Dir;
+  out: Σ;
+}.
+
+Definition TM:Set := St->Σ->option Trans.
+
+Definition ExecState:Set := St*(Z->Σ).
+
+Definition InitES:ExecState := (St0,fun _=>Σ0).
+
+Definition upd(t:(Z->Σ))(o:Σ) :=
+  fun x:Z => if Z.eqb x Z0 then o else t x.
+
+Definition mov(t:(Z->Σ))(d:Dir) :=
+  fun x:Z => t ((x+(Dir_to_Z d))%Z).
+
+Definition step(tm:TM)(st:ExecState): option ExecState :=
+  let (s,t):=st in
+  match tm s (t Z0) with
+  | None => None
+  | Some tr =>
+    let (s',d,o):=tr in
+    Some (s',mov (upd t o) d)
+  end.
+
+Inductive Steps: TM->nat->ExecState->ExecState->Prop :=
+| steps_O tm st:
+  Steps tm O st st
+| steps_S tm n st st0 st1:
+  Steps tm n st st0 ->
+  step tm st0 = Some st1 ->
+  Steps tm (S n) st st1.
+
+Definition HaltsAt(tm:TM)(n:nat)(st:ExecState): Prop :=
+  exists st', Steps tm n st st' /\ step tm st' = None.
+
+End TM.
+
+Definition BB5 := 47176869%N.
+
+Definition BB5_value_statement :=
+  (forall tm n0, HaltsAt Σ tm n0 (InitES Σ Σ0) -> n0 <= N.to_nat BB5) /\
+  (exists tm, HaltsAt Σ tm (N.to_nat BB5) (InitES Σ Σ0)).
+
